Base.thy
@@ -5,6 +5,14 @@ begin
 no_notation Ref.update ("_ := _" 62)
 notation Ref.update ("_ :=\<^sub>R _" 62)
 
+abbreviation contains where
+  "contains x xs \<equiv> x \<in> set xs"
+
+notation contains ("(_/ \<in>\<^sub>L _)" [51, 51] 50)
+
+lemma ent_iff:"A = B \<longleftrightarrow> (B \<Longrightarrow>\<^sub>A A) \<and> (A \<Longrightarrow>\<^sub>A B)"
+  using ent_iffI by auto
+
 lemma htriple_frame_fwd:
   assumes R: "P \<Longrightarrow>\<^sub>A R"
   assumes F: "Ps \<Longrightarrow>\<^sub>A P*F"
@@ -13,17 +21,14 @@ lemma htriple_frame_fwd:
   using assms
   by (metis cons_rule ent_refl fr_refl)
 
-lemma htriple_combine_post: "<P> c <Q> \<Longrightarrow> <P> c <Q'> \<Longrightarrow> <P> c <\<lambda>r. Q r \<and>\<^sub>A Q' r>"
-  unfolding hoare_triple_def
-  by(auto simp: Let_def mod_and_dist)
-
+(* TODO: Probably not needed *)
 lemma htriple_return_entails: "<P> return x <Q> \<Longrightarrow> P \<Longrightarrow>\<^sub>A Q x"
   unfolding hoare_triple_def Let_def entails_def
   using effect_returnI effect_run by fastforce
 
-lemma htriple_return_and: " \<lbrakk><\<Gamma>> return a <\<Gamma>\<^sub>a>; <\<Gamma>> return b <\<Gamma>\<^sub>b>\<rbrakk> \<Longrightarrow> \<Gamma> \<Longrightarrow>\<^sub>A \<Gamma>\<^sub>a a \<and>\<^sub>A \<Gamma>\<^sub>b b"
-  using htriple_return_entails[of \<Gamma> a \<Gamma>\<^sub>a] htriple_return_entails[of \<Gamma> b \<Gamma>\<^sub>b] ent_conjI
-  by auto
+(* TODO: Probably not needed *)
+lemma lookup_fwd: "<A> !a <\<lambda>c. A>"
+  by (smt (verit, del_insts) deconstruct_rules(4) effect_returnI effect_run hoare_triple_def new_addr_refl run_lookup the_state.simps)
 
 method sep_drule uses r = 
   rule ent_frame_fwd[OF r] htriple_frame_fwd[OF r], (assumption+)?, frame_inference
