Cell.thy
@@ -5,9 +5,8 @@ begin
 datatype 'a::"countable" cell = Array "'a array" | Upd nat "'a" "'a cell ref"
 
 derive countable cell
-
-instance cell :: (heap) heap
-   by standard
+ 
+instance cell :: (heap) heap ..
 
 datatype 'a::"countable" cell' = Array' "'a list" | Upd' nat "'a" "'a cell ref"
 
@@ -17,16 +16,7 @@ fun cell_assn where
 | "cell_assn _ _ = false"
 
 lemma cell_assn_array [simp]: "cell_assn (Array' xs) c = (\<exists>\<^sub>Aa. \<up>(c = Array a) * a \<mapsto>\<^sub>a xs)"
-proof(cases c)
-  case (Array x1)
-  then show ?thesis 
-    apply sep_auto 
-    apply (rule ent_iffI)
-    by sep_auto+
-next
-  case Upd
-  then show ?thesis by auto
-qed
+  by(cases c)(auto simp: ent_iff entails_def)
 
 lemma cell_assn_upd [simp]: "cell_assn (Upd' i x p) c = \<up>(c = Upd i x p)"
   by(cases c) auto
