Example_CYK.thy
@@ -1,0 +1,49 @@
+theory Example_CYK
+  imports Hnr_Diff_Arr Hnr_Array "HOL-Library.Code_Target_Nat" Definition_Utils
+begin
+
+datatype ('n, 't) RHS = NonTerminals 'n 'n | Terminal 't 
+
+type_synonym ('n, 't) CNG = "('n \<times> ('n, 't) RHS) list"
+
+(* 
+  1. Write as case on list. How should HNR rule look like for it? 
+     Go via length of (diff-)arr
+  2. How to handle recursion?
+*)
+fun member :: "'a \<Rightarrow> 'a list \<Rightarrow> bool" where 
+  "member a [] = False" 
+| "member a (x#xs) = (x = a \<or> member a xs)"
+
+fun member' :: "'a \<Rightarrow> 'a list \<Rightarrow> bool" where 
+  "member' a xs = (
+    case xs of
+      [] \<Rightarrow> False
+    | x#xs \<Rightarrow> (x = a \<or> member' a xs)
+  )" 
+
+fun match_prods :: "('n, 't) CNG \<Rightarrow> 'n list \<Rightarrow> 'n list \<Rightarrow> 'n list" where 
+  "match_prods [] ls rs = []" 
+| "match_prods ((X, NonTerminals A B)#ps) ls rs = (
+    if member A ls \<and> member B rs 
+    then X # match_prods ps ls rs
+    else match_prods ps ls rs
+  )" 
+| "match_prods ((X, Terminal a)#ps) ls rs = match_prods ps ls rs"
+
+function inner :: "('n, 't) CNG \<Rightarrow> (nat \<times> nat \<Rightarrow> 'n list) \<Rightarrow> nat \<Rightarrow> nat \<Rightarrow> nat \<Rightarrow> 'n list" where
+ "inner G T i k j = (
+    if k < j 
+    then match_prods G (T(i, k)) (T(i + k, j - k)) @ inner G T i (k + 1) j
+    else []
+  )"
+by pat_completeness auto
+termination 
+by(relation "measure(\<lambda>(a, b, c, d, e). e - d)", rule wf_measure, simp)
+
+synth_definition member'_impl is [hnr_rule_diff_arr]: 
+    "hnr (master_assn' (insert (xs, xsi) F)) (\<hole> :: ?'a Heap) ?\<Gamma>' (member' x xs)"
+  apply hnr_diff_arr
+  done
+
+end
