Fold_Assn.thy
@@ -2,42 +2,29 @@ theory Fold_Assn
   imports Base
 begin
 
-abbreviation contains where
-  "contains x xs \<equiv> x \<in> set xs"
-
-notation
-  contains ("(_/ \<in>\<^sub>L _)" [51, 51] 50)
-
 definition fold_assn :: "assn list \<Rightarrow> assn" where
   "fold_assn assns = foldr (*) assns emp"
 
-lemma fold_assn_emp[simp]: "fold_assn [] = emp"
-  unfolding fold_assn_def
-  by simp
+lemma fold_assn_emp [simp]: "fold_assn [] = emp"
+  unfolding fold_assn_def by simp
 
-lemma fold_assn_cons[simp]: "fold_assn (x#xs) = x * fold_assn xs"
-  unfolding fold_assn_def
-  by simp_all
+lemma fold_assn_cons [simp]: "fold_assn (x#xs) = x * fold_assn xs"
+  unfolding fold_assn_def by simp_all
 
 lemma fold_assn_app [simp]: "fold_assn (xs@ys) = fold_assn xs * fold_assn ys"
-  apply(induction xs)
-  by(auto simp: algebra_simps)
+  by(induction xs)(auto simp: algebra_simps)
 
 lemma fold_assn_remove1: "x \<in>\<^sub>L xs \<Longrightarrow> fold_assn xs = x * fold_assn (remove1 x xs)"
-  apply(induction xs)
-  by(auto simp: algebra_simps)
+  by(induction xs)(auto simp: algebra_simps)
 
 lemma fold_assn_false [simp]: "false \<in>\<^sub>L xs \<Longrightarrow> fold_assn xs = false"
-  using fold_assn_remove1
-  by auto
+  using fold_assn_remove1 by auto
 
-lemma fold_assn_emp_remove1: "fold_assn xs = fold_assn (remove1 emp xs)"
-  apply(induction xs)
-  by auto
+lemma fold_assn_emp_remove1 [simp]: "fold_assn (remove1 emp xs) = fold_assn xs"
+  by(induction xs) auto
 
-lemma fold_assn_emp_removeAll: "fold_assn xs = fold_assn (removeAll emp xs)"
-  apply(induction xs)
-  by auto  
+lemma fold_assn_emp_removeAll [simp]: "fold_assn (removeAll emp xs) = fold_assn xs"
+  by(induction xs) auto  
 
 lemma fold_assn_remove1_map: "x \<in>\<^sub>L xs
    \<Longrightarrow> fold_assn (remove1 (f x) (map f xs)) = fold_assn (map f (remove1 x xs))"
